Equivalence under reduction

PDDL-sema/Terms.thy
@@ -1,28 +1,105 @@
 theory Terms
   imports AST1
 begin
-  
+
+  (* this is an equivalence relation *)
   type_synonym 'sym function_interpretation = "'sym term \<rightharpoonup> 'sym term"
 
   fun subterms::"'a term \<Rightarrow> 'a term set" where
     "subterms (Sym x) = {Sym x}"
   | "subterms (Fun f as) = insert (Fun f as) (\<Union> (subterms ` (set as)))"
-  
-  (* Normal forms for terms and interpretations *)
-  inductive nf_fi::"'a function_interpretation \<Rightarrow> bool" 
+
+  inductive nf_fi::"'a function_interpretation \<Rightarrow> bool"
         and nf_term::"'a function_interpretation \<Rightarrow> 'a term \<Rightarrow> bool" where
     "\<lbrakk>\<not>(\<exists>obj. Sym obj \<in> dom fi); 
-        \<forall>(f, a) \<in> Map.graph fi. (\<forall>t \<in> subterms t - {t}. nf_term fi t)  \<and> nf_term fi a\<rbrakk> 
+        \<forall>(l, r) \<in> Map.graph fi. (\<forall>t \<in> subterms l - {l}. nf_term fi t)  \<and> nf_term fi r\<rbrakk> 
       \<Longrightarrow> nf_fi fi"
   | "nf_term fi (Sym _)"
   | "\<lbrakk>nf_fi fi; list_all (nf_term fi) as; fi (Fun f as) = None\<rbrakk> 
       \<Longrightarrow> nf_term fi (Fun f as)"
-  
+
   locale term_eq =
     fixes fi::"'sym function_interpretation"
+  begin
+    inductive reduce::"'sym term \<Rightarrow> 'sym term \<Rightarrow> bool" (infix "\<rightarrow>\<^sub>t" 55) where
+      refl: "t \<rightarrow>\<^sub>t t"
+    | trans: "\<lbrakk>t1 \<rightarrow>\<^sub>t t2; t2 \<rightarrow>\<^sub>t t3\<rbrakk> \<Longrightarrow> t1 \<rightarrow>\<^sub>t t3"
+    | def: "(t1, t2) \<in> Map.graph fi \<Longrightarrow> t1 \<rightarrow>\<^sub>t t2"
+    | app: "list_all2 (\<rightarrow>\<^sub>t) as as' \<Longrightarrow> (Fun f as) \<rightarrow>\<^sub>t (Fun f as')"
+  
+    lemma "reduce = (reduce\<^sup>*\<^sup>*)"
+      apply (rule ext)+
+      subgoal for a b
+        apply (rule iffI)
+         apply (induction rule: reduce.induct)
+        subgoal by (rule rtranclp.rtrancl_refl)
+        subgoal for t t' t2
+          apply (rule rtranclp.rtrancl_into_rtrancl)
+          by assumption+
+        subgoal apply (drule def)
+          apply (rule rtranclp.rtrancl_into_rtrancl)
+           apply (rule rtranclp.rtrancl_refl)
+          by assumption
+        subgoal for as as' f
+          apply (rule rtranclp.rtrancl_into_rtrancl[where b = "Fun f as"])
+           apply (rule rtranclp.rtrancl_refl)
+          apply (rule app)
+          apply (induction rule: list_all2_induct)
+           apply simp
+            by auto
+        apply (induction rule: rtranclp.induct)
+         apply (rule refl)
+        subgoal for a b c
+          apply (rule trans)
+          by simp+
+        done
+      done
+  
+      definition eq::"'sym term \<Rightarrow> 'sym term \<Rightarrow> bool" (infix "=\<^sub>t" 55) where
+        "x =\<^sub>t y \<equiv> ((\<rightarrow>\<^sub>t)\<^sup>=\<^sup>=) x y"
+  end
+  
+  locale decidable_eq = term_eq fi 
+    for fi::"'sym term \<Rightarrow> 'sym term option" +
     assumes "nf_fi fi"
   begin
-    definition "eq \<equiv> equivclp (\<lambda>x y. fi x = Some y)"
-  end
+    fun normalise_term::"'sym term \<Rightarrow> 'sym term" where
+      "normalise_term (Sym s) = (Sym s)"
+    | "normalise_term (Fun f as) = (
+        let as' = map normalise_term as 
+        in (case (fi (Fun f as')) of
+          Some t  \<Rightarrow> t
+        | None    \<Rightarrow> (Fun f as')
+        )
+      )"
 
+  definition decidable_eq::"'sym term \<Rightarrow> 'sym term \<Rightarrow> bool" where
+    "decidable_eq a b \<equiv> (normalise_term a) = (normalise_term b)"
+
+lemma nf_unique:
+  assumes 1: "t \<rightarrow>\<^sub>t t'" "nf_term fi t'"
+      and 2: "t \<rightarrow>\<^sub>t t''" "nf_term fi t''"
+    shows "t' = t''"
+  using assms
+proof (induction rule: reduce.induct)
+  case (refl t)
+  then show ?case sorry
+next
+  case (trans t1 t2 t3)
+  then show ?case sorry
+next
+  case (def t1 t2)
+  then show ?case sorry
+next
+  case (app as as' f)
+  then show ?case sorry
+qed
+
+  
+  lemma normalise_nf: "nf_term fi (normalise_term t)"
+    sorry
+  theorem decidable_eq_correct: "eq a b \<longleftrightarrow> decidable_eq a b"
+    sorry
+  end
+  
 end
